\documentclass{scrartcl}

\usepackage[math]{kurier}
\usepackage[T1]{fontenc}
\renewcommand*{\familydefault}{\sfdefault}
\usepackage{array}

\usepackage{amsmath}
\usepackage{amssymb}
\newcommand{\vect}[1]{\boldsymbol{#1}}
\newcommand{\ten}[1]{\boldsymbol{#1}}
\DeclareMathOperator{\trace}{tr}
\DeclareMathOperator{\sym}{sym}
\newcommand{\tr}{^\intercal}
\newcommand{\dff}{\:\mathrm{d}}

\begin{document}

\section{Definitions}

\begin{tabular}{>{$}r<{$}l}
\hline
\vect{d} & displacement \\
\vect{u} & velocity \\
\vect{\nabla} & del operator \\
\rho & density \\
\mu & first viscosity constant \\
\lambda & second viscosity constant \\
\hline
\end{tabular}
\vspace*{2em}

dyadic product
\[
\ten{a b} = \vect{a} \vect{b}\tr = (a_i b_j)
\]

Frobenius product
\[
\ten{\alpha} : \ten{\beta} = \sum_{i,j} \alpha_{ij} \beta_{ij}
\]

derivatives
\[
u_{i,j} = \frac{\partial u_i}{\partial x_j}
\]

\[
\ten{\epsilon}(\vect{u}) = \sym(\ten{\nabla u}) = 
\frac{1}{2}(\ten{\nabla u} + \ten{\nabla u}\tr)
\]

\[
\trace(\ten{\epsilon}(\vect{u})) = \vect{\nabla} \cdot \vect{u}
\]

inner products
\begin{align*}
(a,b) &= \int_{\Omega} a b \dff\Omega \\
(\vect{a},\vect{b}) &= \int_{\Omega} \vect{a} \cdot \vect{b} \dff\Omega \\
(\ten{\alpha},\ten{\beta}) &= \int_{\Omega} \ten{\alpha} : \ten{\beta} \dff\Omega
\end{align*}

\section{Linear Elasticity}
\[
\ten{\sigma} = 2 \mu \ten{\epsilon}(\vect{d}) +
\lambda \trace(\ten{\epsilon}(\vect{d})) \ten{I}
\]

strong form
\[
\rho \ddot{\vect{d}} - \vect{\nabla} \cdot \ten{\sigma}(\vect{d}) = \vect{f}
\]

weak form
\[
(\rho \ddot{\vect{d}},\vect{b}) + (\ten{\sigma}(\vect{d}),\ten{\epsilon}(\vect{b})) =
(\vect{f},\vect{b}) \qquad \forall \vect{b} \in \vect{V}
\]

strong form
\begin{align*}
\dot{\vect{d}} - \vect{u} = 0 \\
\rho \dot{\vect{u}} - \vect{\nabla} \cdot \ten{\sigma}(\vect{d}) = \vect{f}
\end{align*}

weak form
\begin{align*}
&(\dot{\vect{d}},\vect{b}) - (\vect{u},\vect{b}) = 0 & &\forall \vect{b} \in \vect{V} \\
&(\rho \dot{\vect{u}},\vect{v}) + (\ten{\sigma}(\vect{d}),\ten{\epsilon}(\vect{v})) =
(\vect{f},\vect{v}) & &\forall \vect{v} \in \vect{V}
\end{align*}

time discretization
\begin{align*}
&\left(\frac{\vect{d}}{\Delta t},\vect{b}\right) - (\vect{u},\vect{b}) =
\left(\frac{\vect{d}_0}{\Delta t},\vect{b} \right) & &\forall \vect{b} \in \vect{V} \\
&\left(\frac{\rho \vect{u}}{\Delta t},\vect{v}\right)
+ (\ten{\sigma}(\vect{d}),\ten{\epsilon}(\vect{v})) =
\left(\frac{\vect{u}_0}{\Delta t} + \vect{f},\vect{v}\right) & &\forall \vect{v} \in \vect{V}
\end{align*}

\begin{align*}
&(\vect{d},\vect{b}) - \Delta t (\vect{u},\vect{b}) =
(\vect{d}_0,\vect{b}) & &\forall \vect{b} \in \vect{V} \\
&(\vect{u},\vect{v}) + \Delta t(\ten{\sigma}(\vect{d}),\ten{\epsilon}(\vect{v})) =
(\vect{u}_0 + \Delta t\vect{f},\vect{v}) & &\forall \vect{v} \in \vect{V}
\end{align*}

\begin{align*}
&(\vect{d},\vect{b}) - \Delta t (\vect{u},\vect{b}) =
(\vect{d}_0,\vect{b}) & &\forall \vect{b} \in \vect{V} \\
&( \rho \vect{u},\vect{v}) + \Delta t^2 (\ten{\sigma}(\vect{u}),\ten{\epsilon}(\vect{v})) =
(\vect{u}_0 + \Delta t\vect{f},\vect{v}) - \Delta t (\ten{\sigma}(\vect{d_0}),\ten{\epsilon}(\vect{v}))
& &\forall \vect{v} \in \vect{V}
\end{align*}

\[
(\ten{\sigma}(\vect{u}),\ten{\epsilon}(\vect{v})) = 
2\mu (\ten{\epsilon}(\vect{u}),\ten{\epsilon}(\vect{v})) +
\lambda (\trace(\ten{\epsilon}(\vect{u})),\trace(\ten{\epsilon}(\vect{v})))
\]

\subsection{2D Cartesian coordinates}

\[
\ten{\nabla u} =
\begin{pmatrix}
u_{0,0} & u_{1,0} \\
u_{0,1} & u_{1,1}
\end{pmatrix}
\]

\[
\ten{\epsilon}(\vect{u}) =
\begin{pmatrix}
u_{0,0} & \frac{1}{2}(u_{1,0} + u_{0,1}) \\
\frac{1}{2}(u_{1,0} + u_{0,1}) & u_{1,1}
\end{pmatrix}
\]

\[
\vect{\nabla} \cdot \vect{u} = u_{0,0} + u_{1,1}
\]

\begin{align*}
2(\ten{\epsilon}(\vect{u}), \ten{\epsilon}(\vect{v})) =& \\
&2 u_{0,0} v_{0,0} + u_{0,1} v_{0,1} \\
&+ u_{1,0} v_{0,1} \\
&+ u_{0,1} v_{1,0} \\
&+ u_{1,0} v_{1,0} + 2 u_{1,1} v_{1,1}
\end{align*}

\begin{align*}
(\vect{\nabla} \cdot \vect{u}, \vect{\nabla} \cdot \vect{v}) =& \\
& u_{0,0} v_{0,0} \\
&+ u_{1,1} v_{0,0} \\
&+ u_{0,0} v_{1,1} \\
&+ u_{1,1} v_{1,1}
\end{align*}

\subsection{Cylindrical coordinates}

coordinates
\begin{align*}
&r = x_0 & &\theta = x_1 & &z = x_2
\end{align*}

time derivative
\[
\dot{\vect{u}} = ( \dot{u}_0 - u_1 \dot{x}_1, \dot{u}_1 
+ u_0 \dot{x}_1, \dot{u}_2 )
\]

strain tensor
\[
\ten{\epsilon}(\vect{u}) = 
\begin{pmatrix}
u_{0,0} & \frac{1}{2}(\frac{1}{x_0}u_{0,1} + u_{1,0} + \frac{1}{x_0}u_1) &
\frac{1}{2}(u_{0,2} + u_{2,0}) \\
\frac{1}{2}(\frac{1}{x_0}u_{0,1} + u_{1,0} + \frac{1}{x_0}u_1) &
\frac{1}{x_0}(u_{1,1} + u_0) & \frac{1}{2}(u_{1,2} + \frac{1}{x_0}u_{2,1}) \\
\frac{1}{2}(u_{0,2} + u_{2,0}) & \frac{1}{2}(u_{1,2} + \frac{1}{x_0}u_{2,1}) &
u_{2,2} 
\end{pmatrix}
\]

divergence
\[
\vect{\nabla} \cdot \vect{u} = u_{0,0} + \frac{1}{x_0}u_0 + \frac{1}{x_0}u_{1,1}
+ u_{2,2}
\]

\subsubsection{axisymmetry}

\begin{align*}
&\theta = 0 & &f_{,\theta} = 0 & & z = x_1
\end{align*}

time derivative
\[
\dot{\vect{u}} = ( \dot{u}_0, \dot{u}_1 )
\]

strain tensor
\[
\ten{\epsilon}(\vect{u}) = 
\begin{pmatrix}
u_{0,0} & 0 & \frac{1}{2}(u_{0,1} + u_{1,0}) \\
0 & \frac{1}{x_0}u_0 & 0 \\
\frac{1}{2}(u_{0,1} + u_{1,0}) & 0 & u_{1,1} 
\end{pmatrix}
\]

divergence
\[
\vect{\nabla} \cdot \vect{u} = u_{0,0} + \frac{1}{x_0}u_0 + u_{1,1}
\]

\begin{align*}
2(\ten{\epsilon}(\vect{u}), \ten{\epsilon}(\vect{v})) =& \\
&\frac{2}{x_0^2}u_0 v_0 + 2 u_{0,0} v_{0,0} + u_{0,1} v_{0,1} \\
&+ u_{1,0} v_{0,1} \\
&+ u_{0,1} v_{1,0} \\
&+ u_{1,0} v_{1,0} + 2 u_{1,1} v_{1,1}
\end{align*}

\begin{align*}
(\vect{\nabla} \cdot \vect{u}, \vect{\nabla} \cdot \vect{v}) =& \\
& u_{0,0} v_{0,0} + \frac{1}{x_0} u_0 v_{0,0} 
+ \frac{1}{x_0} u_{0,0} v_0 + \frac{1}{x_0^2} u_0 v_0 \\
&+ u_{1,1} v_{0,0} + \frac{1}{x_0} u_{1,1} v_0 \\
&+ u_{0,0} v_{1,1} + \frac{1}{x_0} u_0 v_{1,1} \\
&+ u_{1,1} v_{1,1}
\end{align*}

\end{document}

